TM/Combinators/Combinators.v
@@ -1,5 +1,5 @@
 (* Export the submodules *)
-Require Export Match If SequentialComposition While.
+Require Export Match If SequentialComposition While Mirror.
 
 
 
