TM/Compound/CopySymbols.v
@@ -1,9 +1,8 @@
 Require Import TM.Prelim.
 Require Import TM.Basic.Mono.
 Require Import TM.Combinators.Combinators.
-Require Import TM.Mirror.
 Require Import TM.Compound.TMTac TM.Compound.Multi.
-Require Import TM.LiftMN.
+Require Import TM.Lifting.LiftTapes.
 
 Require Import FunInd.
 Require Import Recdef.
@@ -29,9 +28,9 @@ Section CopySymbols.
                (* First write the read symbol to tape 1 *)
                if f x
                then (* found the symbol: write it to tape 1; break and return *)
-                 Inject (Return (Write (g x)) (Some tt)) [|Fin.FS Fin.F1|]
+                 LiftTapes (Return (Write (g x)) (Some tt)) [|Fin.FS Fin.F1|]
                else (* wrong symbol: write it to tape 1 and move both tapes right and continue *)
-                 Inject (Return (Write (g x)) tt) [|Fin.FS Fin.F1|];;
+                 LiftTapes (Return (Write (g x)) tt) [|Fin.FS Fin.F1|];;
                  Return (MovePar R R) (None)
              | _ => Return Nop (Some tt) (* there is no such symbol, break and return *)
              end).
@@ -84,12 +83,12 @@ End Test.
   Proof.
     eapply RealiseIn_monotone.
     {
-      unfold M1. eapply Match_RealiseIn. cbn. eapply Inject_RealiseIn; [vector_dupfree| eapply ReadChar_Sem].
+      unfold M1. eapply Match_RealiseIn. cbn. eapply LiftTapes_RealiseIn; [vector_dupfree| eapply ReadChar_Sem].
       instantiate (2 := fun o : option sig => match o with Some x => if f x then _ else _ | None => _ end).
       intros [ | ]; cbn.
       - destruct (f e); swap 1 2.
-        + eapply Seq_RealiseIn. eapply Inject_RealiseIn; [vector_dupfree | eapply Write_Sem]. apply Return_RealiseIn. eapply MovePar_Sem.
-        + cbn. eapply Inject_RealiseIn; [vector_dupfree | eapply Return_RealiseIn, Write_Sem].
+        + eapply Seq_RealiseIn. eapply LiftTapes_RealiseIn; [vector_dupfree | eapply Write_Sem]. apply Return_RealiseIn. eapply MovePar_Sem.
+        + cbn. eapply LiftTapes_RealiseIn; [vector_dupfree | eapply Return_RealiseIn, Write_Sem].
       - cbn. eapply RealiseIn_monotone'. apply Return_RealiseIn. eapply Nop_Sem. omega.
     }
     {
